wip on monadic logging memory

src/Minimal.v
@@ -6,6 +6,7 @@ Require Import riscv.RiscvBitWidths.
 Require Import riscv.util.Monads.
 Require Import riscv.Decode.
 Require Import riscv.Memory. (* should go before Program because both define loadByte etc *)
+Require Import riscv.MonadicMemory.
 Require Import riscv.Program.
 Require Import riscv.Execute.
 Require Import riscv.util.PowerFunc.
@@ -20,7 +21,9 @@ Section Riscv.
 
   Context {Mem: Set}.
 
-  Context {MemIsMemory: Memory Mem (word wXLEN)}.
+  Context {MemIsMem: Memory Mem (word wXLEN)}.
+
+  Context {MemIsMonadicMemory: MonadicMemory (OState Mem) (word wXLEN)}.
 
   Definition Register := Z.
 
@@ -30,32 +33,40 @@ Section Riscv.
     name := Z
   |}.
 
-  Record RiscvMachine := mkRiscvMachine {
-    machineMem: Mem;
+  Record RiscvMachineCore := mkRiscvMachineCore {
     registers: Register -> word wXLEN;
     pc: word wXLEN;
     nextPC: word wXLEN;
     exceptionHandlerAddr: MachineInt;
   }.
 
-  Definition with_machineMem me ma :=
-    mkRiscvMachine me ma.(registers) ma.(pc) ma.(nextPC) ma.(exceptionHandlerAddr).
+  Record RiscvMachine := mkRiscvMachine {
+    core: RiscvMachineCore;
+    machineMem: Mem;
+  }.
+
   Definition with_registers r ma :=
-    mkRiscvMachine ma.(machineMem) r ma.(pc) ma.(nextPC) ma.(exceptionHandlerAddr).
+    mkRiscvMachine (mkRiscvMachineCore
+        r ma.(core).(pc) ma.(core).(nextPC) ma.(core).(exceptionHandlerAddr))
+        ma.(machineMem).
   Definition with_pc p ma :=
-    mkRiscvMachine ma.(machineMem) ma.(registers) p ma.(nextPC) ma.(exceptionHandlerAddr).
+    mkRiscvMachine (mkRiscvMachineCore
+        ma.(core).(registers) p ma.(core).(nextPC) ma.(core).(exceptionHandlerAddr))
+        ma.(machineMem).
   Definition with_nextPC npc ma :=
-    mkRiscvMachine ma.(machineMem) ma.(registers) ma.(pc) npc ma.(exceptionHandlerAddr).
+    mkRiscvMachine (mkRiscvMachineCore
+        ma.(core).(registers) ma.(core).(pc) npc ma.(core).(exceptionHandlerAddr))
+        ma.(machineMem).
   Definition with_exceptionHandlerAddr eh ma :=
-    mkRiscvMachine ma.(machineMem) ma.(registers) ma.(pc) ma.(nextPC) eh.
+    mkRiscvMachine (mkRiscvMachineCore
+        ma.(core).(registers) ma.(core).(pc) ma.(core).(nextPC) eh)
+        ma.(machineMem).
+  Definition with_machineMem m ma :=
+    mkRiscvMachine ma.(core) m.
 
-  Definition liftLoad{sz: nat}(f: Mem -> word wXLEN -> word sz)(a: word wXLEN)
-    : OState RiscvMachine (word sz) :=
-    m <- gets machineMem; Return (f m a).
-
-  Definition liftStore{sz: nat}(f: Mem -> word wXLEN -> word sz -> Mem)
-    (a: word wXLEN)(v: word sz) : OState RiscvMachine unit :=
-    m <- get; let mem' := f m.(machineMem) a v in put (with_machineMem mem' m).
+  Instance MM: MonadicMemory (OState RiscvMachine) (word wXLEN).
+    (* TODO lift MemIsMonadicMemory *)
+  Admitted.
 
   Instance IsRiscvMachine: RiscvState (OState RiscvMachine) :=
   {|
@@ -63,7 +74,7 @@ Section Riscv.
         if dec (reg = Register0) then
           Return $0
         else
-          machine <- get; Return (machine.(registers) reg);
+          machine <- get; Return (machine.(core).(registers) reg);
 
       setRegister := fun (reg: name) v =>
         if dec (reg = Register0) then
@@ -72,33 +83,35 @@ Section Riscv.
           machine <- get;
           let newRegs := (fun reg2 => if dec (reg = reg2)
                                       then v
-                                      else machine.(registers) reg2) in
+                                      else machine.(core).(registers) reg2) in
           put (with_registers newRegs machine);
 
-      getPC := gets pc;
+      getPC := machine <- get; Return machine.(core).(pc);
 
       setPC := fun newPC =>
         machine <- get;
         put (with_nextPC newPC machine);
 
-      loadByte   := liftLoad Memory.loadByte;
-      loadHalf   := liftLoad Memory.loadHalf;
-      loadWord   := liftLoad Memory.loadWord;
-      loadDouble := liftLoad Memory.loadDouble;
+      loadByte   := MonadicMemory.loadByte;
+      loadHalf   := MonadicMemory.loadHalf;
+      loadWord   := MonadicMemory.loadWord;
+      loadDouble := MonadicMemory.loadDouble;
 
-      storeByte   := liftStore Memory.storeByte;
-      storeHalf   := liftStore Memory.storeHalf;
-      storeWord   := liftStore Memory.storeWord;
-      storeDouble := liftStore Memory.storeDouble;
+      storeByte   := MonadicMemory.storeByte;
+      storeHalf   := MonadicMemory.storeHalf;
+      storeWord   := MonadicMemory.storeWord;
+      storeDouble := MonadicMemory.storeDouble;
 
       step :=
         m <- get;
-        put (with_nextPC (m.(nextPC) ^+ $4) (with_pc m.(nextPC) m));
+        put (with_nextPC (m.(core).(nextPC) ^+ $4) (with_pc m.(core).(nextPC) m));
 
       getCSRField_MTVecBase :=
-        gets exceptionHandlerAddr;
+        machine <- get;
+        Return machine.(core).(exceptionHandlerAddr);
 
       endCycle A := fun _ => None; (* TODO that's wrong, TODO get monad transformer stuff right *)
+
   |}.
 
   (* Puts given program at address 0, and makes pc point to beginning of program, i.e. 0.
@@ -107,11 +120,8 @@ Section Riscv.
      which might contain any undefined garbage values, so the compiler correctness proof
      will show that the program is correct even then, i.e. no initialisation of the registers
      is needed. *)
-  Definition putProgram(prog: list (word 32))(m: RiscvMachine): RiscvMachine :=
-    match m with
-    | mkRiscvMachine m regs _ _ eh =>
-        mkRiscvMachine (store_word_list prog $0 m) regs $0 $4 eh
-    end.
+  Definition putProgram(prog: list (word 32))(ma: RiscvMachine): RiscvMachine :=
+    with_pc $0 (with_nextPC $4 (with_machineMem (store_word_list prog $0 ma.(machineMem)) ma)).
 
 End Riscv.
 
