src/LoggingMemory.v
@@ -1,0 +1,68 @@
+Require Import Coq.Lists.List.
+Import ListNotations.
+Require Import bbv.Word.
+Require Import riscv.Memory.
+Require Import riscv.MonadicMemory.
+Require Import riscv.util.Monads.
+
+Inductive TraceEvent{a: Set}: Set :=
+| Trace_loadByte   : a -> word  8 -> TraceEvent
+| Trace_loadHalf   : a -> word 16 -> TraceEvent
+| Trace_loadWord   : a -> word 32 -> TraceEvent
+| Trace_loadDouble : a -> word 64 -> TraceEvent
+| Trace_storeByte  : a -> word  8 -> TraceEvent
+| Trace_storeHalf  : a -> word 16 -> TraceEvent
+| Trace_storeWord  : a -> word 32 -> TraceEvent
+| Trace_storeDouble: a -> word 64 -> TraceEvent.
+
+Arguments TraceEvent: clear implicits.
+
+Definition LoggingMemory(m a: Set) := (m * list (TraceEvent a))%type.
+
+Definition log{M A: Set}(m: LoggingMemory M A)(e: TraceEvent A): LoggingMemory M A :=
+  (fst m, snd m ++ [e]).
+
+Definition myInst M A: Monad (State (LoggingMemory M A)) := State_Monad _.
+
+Existing Instance myInst.
+
+Instance StateLoggingMemory_is_MonadicMemory(M A: Set){MM: Memory M A}:
+  MonadicMemory (State (LoggingMemory M A)) A :=
+{|
+  loadByte a :=
+     m <- StateM.get;
+     let r := Memory.loadByte (fst m) a in
+     StateM.put (log m (Trace_loadByte a r));;
+     Return r;
+  loadHalf a :=
+     m <- StateM.get;
+     let r := Memory.loadHalf (fst m) a in
+     StateM.put (log m (Trace_loadHalf a r));;
+     Return r;
+  loadWord a :=
+     m <- StateM.get;
+     let r := Memory.loadWord (fst m) a in
+     StateM.put (log m (Trace_loadWord a r));;
+     Return r;
+  loadDouble a :=
+     m <- StateM.get;
+     let r := Memory.loadDouble (fst m) a in
+     StateM.put (log m (Trace_loadDouble a r));;
+     Return r;
+  storeByte a v :=
+     m <- StateM.get;
+     let m' := Memory.storeByte (fst m) a v in
+     StateM.put (log (m', snd m) (Trace_storeByte a v));
+  storeHalf a v :=
+     m <- StateM.get;
+     let m' := Memory.storeHalf (fst m) a v in
+     StateM.put (log (m', snd m) (Trace_storeHalf a v));
+  storeWord a v :=
+     m <- StateM.get;
+     let m' := Memory.storeWord (fst m) a v in
+     StateM.put (log (m', snd m) (Trace_storeWord a v));
+  storeDouble a v :=
+     m <- StateM.get;
+     let m' := Memory.storeDouble (fst m) a v in
+     StateM.put (log (m', snd m) (Trace_storeDouble a v));
+|}.
